added a rule for triple gates, oracles, grover algorithm and a template for deutsch algorithm

FY/Grover.v
@@ -7,13 +7,61 @@ From FY Require Export Semantics.
 From FY Require Export Assertion.
 From FY Require Export Logic.
 
+Definition X : string := "X".
+Definition Y0 : string := "Y0".
+Definition Y1 : string := "Y1".
+Definition Y2 : string := "Y2".
+Definition K : string := "K".
+
+Definition U100 : Matrix 8 8 := l2M [[1;0;0;0;0;0;0;0];
+                                     [0;1;0;0;0;0;0;0];
+                                     [0;0;1;0;0;0;0;0];
+                                     [0;0;0;-1%C;0;0;0;0];
+                                     [0;0;0;0;1;0;0;0];
+                                     [0;0;0;0;0;1;0;0];
+                                     [0;0;0;0;0;0;1;0];
+                                     [0;0;0;0;0;0;0;1]].
+
+Lemma U100W: U100 × ∣1,0,0⟩ = -1 * ∣1,0,0⟩.
+Proof.
+Admitted.
+
+(*TODO: not complete*)
+Lemma U100NW: forall (w: Vector 8), w <> ∣1,0,0⟩ -> U100 × w = w.
+Proof.
+Admitted.
+
+Definition G := GOracle 8 U100.
+
+Lemma kron_I_1: kron (I 2) (I 1) = I 2.
+Proof.
+Admitted.
+
 Definition GROVER : com :=
-  <{}>.
+  <{
+    q 0 := 0;
+    q 1 := 0;
+    q 2 := 0;
+    q 0 *=1 GH;
+    q 1 *=1 GH;
+    q 2 *=1 GH;
+    K :=c (3 % nat); (* 3 ~ sqrt(8) *)
+    X :=c (0 % nat);
+    while X <= K do
+      q 0 1 2 *=3 G;
+      X :=c (X + 1%nat)
+    end;
+    Y0 :=measQ 0;
+    Y1 :=measQ 1;
+    Y2 :=measQ 2
+  }>.
 
 Print GROVER.
 
-Theorem final_state: ceval GROVER [(( _ !-> 0%nat), I 1)] [(( _ !-> 0%nat), I 1)] .
+Theorem final_state: ceval GROVER [(( _ !-> 0%nat), I 1)] [(( X !-> 3%nat ; K !-> 3%nat ; Y0 !-> 0%nat ; Y1 !-> 0%nat ;Y2 !-> 1%nat; _ !-> 0%nat), ∣0⟩⟨0∣ )] .
 Proof.
+  eapply E_Seq.
+  apply E_Init.
 Admitted.
 
 
