FY/Deutsch.v
@@ -1,0 +1,26 @@
+From Coq Require Import Strings.String.
+From Coq Require Import Lists.List.
+Import ListNotations.
+From FY Require Export Utils.
+From FY Require Export Syntax.
+From FY Require Export Semantics.
+From FY Require Export Assertion.
+From FY Require Export Logic.
+
+Definition X : string := "X".
+Definition Y : string := "Y".
+Definition K : string := "K".
+
+Definition DJ : com :=
+  <{
+  }>.
+
+Print DJ.
+
+Theorem final_state: ceval DJ [(( _ !-> 0%nat), I 1)] [(( _ !-> 0%nat), I 1)] .
+Proof.
+Admitted.
+
+
+
+
